---
Title: Math Formulas
Date: 05-11-2023 8:28 PM
---

# Math Formulas

### 1. Standard Angle Value
||$0^{\circ}$|$30^{\circ}$|$45^{\circ}$|$60^{\circ}$|$90^{\circ}$|$120^{\circ}$|$240^{\circ}$|
|--|--|--|--|--|--|--|--|
|sin | 0 | $\frac{1}{2}$ | $\frac{1}{\sqrt{2}}$ | $\frac{\sqrt{3}}{2}$ | 1 | $\frac{\sqrt{3}}{2}$ | - $\frac{\sqrt{3}}{2}$ |
|cos | 1 | $\frac{\sqrt{3}}{2}$ | $\frac{1}{\sqrt{2}}$ | $\frac{1}{2}$ | 0 | - $\frac{1}{2}$ | - $\frac{1}{2}$ |
|tan|0| $\frac{1}{\sqrt{3}}$ | 1 | $\sqrt{3}$ | undefined | - $\sqrt{3}$ | $\sqrt{3}$ |


$sin^{-1}1 = \frac{\pi}{2}$  
$cos^{-1}1 = 0$  
$tan^{-1}1 = \frac{\pi}{4}$


### 2. Fundamental Relation
$sin^{2}A + cos^{2}A = 1$  
$sec^{2}A - tan^{2}A = 1$  
$cosec^{2}A - cotA = 1$


### 3. Fundamental Theorem
sin(A+B) = sinAcosB + cosAsinB  
sin(A-B) = sinAcosB - cosAsinB  
cos(A+B) = cosAcosB - sinAsinB  
cos(A-B) = cosAcosB + sinAsinB


### 4. Division Method
$tan(A+B) = \frac{tanA + tanB} {1 - tanAtanB}$  
$tan(A-B) = \frac{tanA - tanB} {1 + tanAtanB}$  
$cot(A+B) = \frac{cotAcotB - 1} {cotB + cotA}$  
$cot(A-B) = \frac{cotAcotB + 1} {cotB - cotA}$  


### 5. Multiplication Method
$$
\begin{align*}
sin(A+B)sin(A-B) = sin^{2}A - sin^{2}B \\
= cos^{2}B - cos^{2}A
\end{align*}
$$

$$
\begin{align*}
cos(A+B)cos(A-B) = cos^{2}A - sin^{2}B \\
= cos^{2}B - sin^{2}A
\end{align*}
$$

$$
\begin{align*}
tan(A+B)tan(A-B) = \frac{tan^{2}A-tan^{2}B}{1-tan^{2}Atan^{2}B}
\end{align*}
$$

$$
\begin{align*}
cot(A+B)cot(A-B) = \frac{1- cot^{2}Acot^{2}B}{cot^{2}A - cot^{2}B}
\end{align*}
$$


### 6. Addition & Subtraction
sin(A+B) + sin(A-B) = 2sinAcosB  
sin(A+B) - sin(A-B) = 2cosAsinB  
cos(A+B) + cos(A-B) = 2cosAcosB  
cos(A-B) - cos(A-B) = 2sinAsinB


### 7. Transformation Method
$sinC + sinD = 2sin\frac{C+D}{2}cos\frac{C-D}{2}$  
$sinC - sinD = 2cos\frac{C+D}{2}sin\frac{C-D}{2}$  
$cosC + cosD = 2cos\frac{C+D}{2}cos\frac{C-D}{2}$  
$cosC - cosD = 2sin\frac{C+D}{2}sin\frac{D-C}{2}$



### 8. Double Angle Formula
sin2A = 2sinAcosA  
$sin2A = \frac{2tanA}{1 + tan^{2}A}$  

$cos2A = cos^{2}A - sin^{2}A$  
$cos2A = 2cos^{2} - 1$  
$cos2A = 1- 2sin^{2}$  
$cos2A = \frac{1 - tan^{2}A}{1 + tan^{2}A}$  

$tan2A = \frac{2tanA}{1 - tan^{2}A}$  
$cot2A = \frac{cot^{2}A - 1}{2cotA}$

$sin^{2}A = \frac{1}{2}(1-cos2A)$  
$cos^{2}A = \frac{1}{2}(1+cos2A)$  
$sinAcosA = \frac{1}{2}(sin2A)$


### 9. Triple Angle Formula
$sin3A = 3sinA - 4sin^{3}A$  
$cos3A = 4cos^{3}A - 3cosA$  
$tan3A = \frac{3tanA - tan^{3}A}{1-3tan^{2}A}$  
$cot3A = \frac{3cotA - cot^{3}A}{1-3cot^{2}A}$  

$sin^{3}A = \frac{1}{4}(3sinA - sin3A)$  
$cos^{3}A = \frac{1}{4}(3cosA + cos3A)$  
$tan^{3}A = 3tanA + tan3A(3tan^{2}A - 1)$  
$cot^{3}A = 3cotA + cot3A(3cot^{2}A - 1)$  

### 10. Equation



### 11. Inverse Function
$tan^{-1}x \pm tan^{-1}y = tan^{-1}\frac{x \pm y}{1 \mp xy}$  
$sin^{-1}x \pm sin^{-1}y = sin^{-1}(x\sqrt{1-y^{2}} \pm y\sqrt{1-x^{2}})$  
$cos^{-1}x \pm cos^{-1}y = cos^{-1} \{xy \mp \sqrt{(1-x^{2})(1-y^{2})} \}$  


$sin^{-1}\frac{2x}{1+x^{2}} = 2tan^{-1}x$  
$cos^{-1}\frac{1-x^{2}}{1+x^{2}} = 2tan^{-1}x$  
$tan^{-1}\frac{2x}{1-x^{2}} = 2tan^{-1}x$


### 12. Properties of Triangles
$\frac{a}{sinA} = \frac{b}{sinB} = \frac{c}{sinC} = 2R$  
$cosA = \frac{b^{2}+c^{2}-a^{2}}{2bc}$

$a = bcosC + ccosB$  
$b = ccosA + acosC$  
$c = acosB + bcosA$  




























